verify spawn and join for lib/spawn

theories/typing/lib/spawn.v
@@ -48,7 +48,7 @@ Section spawn.
   Global Instance join_handle_type_contractive {𝔄} : TypeContractive (@join_handle 𝔄).
   Proof.
     split; [by apply type_lft_morphism_id_like|done| |done]=>/= *.
-    rewrite /join_future. Opaque box. do 15 f_equiv. by apply box_type_contractive.
+    rewrite /join_future. do 15 f_equiv. by apply box_type_contractive.
   Qed.
 
   Global Instance join_handle_send {𝔄} (ty: type 𝔄) : Send (join_handle ty).
@@ -93,73 +93,73 @@ Section spawn.
     eqtype E L (join_handle ty) (join_handle ty') (forward_pred f) (forward_pred g).
   Proof. move=> [??]. split; by apply join_handle_subtype. Qed.
 
-(*
-  Definition spawn (call_once : val) : val :=
+  Definition spawn (call_once: val) : val :=
     fn: ["f"] :=
       let: "call_once" := call_once in
-      let: "join" := spawn [λ: ["c"],
-                            letcall: "r" := "call_once" ["f":expr] in
-                            finish ["c"; "r"]] in
-      letalloc: "r" <- "join" in
+      let: "j" := spawn
+        [λ: ["c"], letcall: "r" := "call_once" ["f"] in finish ["c"; "r"]] in
+      letalloc: "r" <- "j" in
       return: ["r"].
 
-  Lemma spawn_type fty retty call_once `(!Send fty, !Send retty) :
-    typed_val call_once (fn(∅; fty) → retty) → (* fty : FnOnce() -> retty, as witnessed by the impl call_once *)
+  Lemma spawn_type {𝔄 𝔅} (Φ: pred' 𝔅) tr (fty: type 𝔄) (retty: type 𝔅)
+      call_once `{!Send fty, !Send retty} :
+    typed_val call_once (fn(∅; fty) → retty) tr →
     let E ϝ := ty_outlives_E fty static ++ ty_outlives_E retty static in
-    typed_val (spawn call_once) (fn(E; fty) → join_handle retty).
+    typed_val (spawn call_once) (fn(E; fty) → join_handle retty)
+      (λ post f, tr Φ f ∧ post Φ).
   Proof.
-    intros Hf ? E L. iApply type_fn; [solve_typing..|]. iIntros "/= !>".
-      iIntros (_ ϝ ret arg). inv_vec arg=>env. simpl_subst.
-    iApply type_let; [apply Hf|solve_typing|]. iIntros (f'). simpl_subst.
-    iApply (type_let _ _ _ _ ([f' ◁ _; env ◁ _])
-                     (λ j, [j ◁ join_handle retty])); try solve_typing; [|].
-    { (* The core of the proof: showing that spawn is safe. *)
-      iIntros (tid) "#LFT #TIME #HE $ $ [Hf' [Henv _]]". rewrite !tctx_hasty_val [fn _]lock.
-      iApply wp_fupd. iApply (spawn_spec _ (join_inv retty) with "[-]"); last first.
-      { iIntros "!> *". rewrite tctx_interp_singleton tctx_hasty_val.
-        iIntros "?". iExists 0%nat. iMod persistent_time_receipt_0 as "$". by iFrame. }
-      simpl_subst. iIntros (c) "Hfin". iMod na_alloc as (tid') "Htl". wp_let. wp_let.
-      iDestruct "Hf'" as (?) "[_ Hf']".
-      unlock. iApply (type_call_iris _ [] () [_] with "LFT TIME HE Htl [] Hf' [Henv]");
-      (* The `solve_typing` here shows that, because we assume that `fty` and `retty`
-         outlive `static`, the implicit requirmeents made by `call_once` are satisifed. *)
-        [solve_typing|iApply (lft_tok_static 1%Qp)| |].
-      - iDestruct "Henv" as (?) "?".
-        rewrite big_sepL_singleton tctx_hasty_val send_change_tid. eauto.
-      - iIntros (r depth') "Htl _ #Hdepth' Hret".
-        wp_rec. iApply (finish_spec with "[$Hfin Hret]"); last auto.
-        iIntros (?). rewrite tctx_hasty_val. iExists _. iFrame "Hdepth'".
-        by iApply @send_change_tid. }
-    iIntros (v). simpl_subst.
-    iApply type_new; [solve_typing..|]. iIntros (r). simpl_subst.
-    iApply type_assign; [solve_typing..|].
-    iApply type_jump; solve_typing.
+    move=> ??. eapply type_fn; [solve_typing|]=>/= _ ??[f[]]. simpl_subst.
+    via_tr_impl.
+    { iApply type_val; [done|]. intro_subst_as (c).
+      iApply (type_let' +[c ◁ fn(_;_)→_; f ◁ _] (λ j, +[j ◁ join_handle retty])
+        (λ post '-[tr'; f], tr' Φ -[f] ∧ post -[Φ])).
+      { iIntros (??(?&?&[])) "LFT TIME PROPH UNIQ E Na L (c & f &_) #Obs".
+        iMod persistent_time_receipt_0 as "⧖".
+        iApply (spawn_spec _ (join_future retty Φ) with "[- ⧖ Na L]"); last first.
+        { iIntros "!> % join". iExists -[const Φ]. iFrame "Na L".
+          iSplit; [|by iApply proph_obs_impl; [|done]=>/= ?[_ ?]]. iSplitL; [|done].
+          rewrite tctx_hasty_val. iExists _. iFrame "⧖". iExists _. by iFrame. }
+        iIntros (?) "/= fin". do 2 wp_let. iMod na_alloc as (tid') "Na".
+        iApply (type_call_iris (𝔄l:=[_]) () -[_] [] 1%Qp (const _) with
+          "LFT TIME PROPH UNIQ E Na [] c [f] [Obs]"); [solve_typing|solve_typing|..].
+        { iApply lft_tok_static. }
+        { rewrite/= right_id !tctx_hasty_val. iDestruct "f" as (?) "[??]".
+          rewrite send_change_tid. iExists _. iFrame. }
+        { by iApply proph_obs_impl; [|done]=>/= [?[? _]]. }
+        iClear "Obs". iIntros (??) "Na _ ret Obs". wp_rec.
+        iApply (finish_spec with "[$fin ret Obs]"); [|done].
+        rewrite tctx_hasty_val. iDestruct "ret" as (?) "[⧖ ?]".
+        iIntros (?). iExists _, _. iFrame "Obs ⧖". by rewrite send_change_tid. }
+      intro_subst. iApply type_letalloc_1; [solve_extract|done|]. intro_subst.
+      iApply type_jump; [solve_typing|solve_extract|solve_typing]. }
+    by move=>/= ?[?[]].
   Qed.
 
-  Definition join : val :=
-    fn: ["c"] :=
-      let: "c'" := !"c" in
-      let: "r" := spawn.join ["c'"] in
-      delete [ #1; "c"];; return: ["r"].
+  Definition join: val :=
+    fn: ["bj"] :=
+      let: "j" := !"bj" in delete [ #1; "bj"];;
+      let: "r" := spawn.join ["j"] in
+      return: ["r"].
 
-  Lemma join_type retty :
-    typed_val join (fn(∅; join_handle retty) → retty).
+  Lemma join_type {𝔄} (retty: type 𝔄) :
+    typed_val join (fn(∅; join_handle retty) → retty)
+      (λ post '-[Φ], ∀a: 𝔄, Φ a → post a).
   Proof.
-    intros E L. iApply type_fn; [solve_typing..|]. iIntros "/= !>".
-      iIntros (_ ϝ ret arg). inv_vec arg=>c. simpl_subst.
-    iApply type_deref; [solve_typing..|]. iIntros (c'); simpl_subst.
-    iApply (type_let _ _ _ _ ([c' ◁ _])
-                             (λ r, [r ◁ box retty])); try solve_typing; [|].
-    { iIntros (tid) "#LFT #TIME _ $ $".
-      rewrite tctx_interp_singleton tctx_hasty_val. iIntros "Hc".
-      iDestruct "Hc" as (depth) "[Hdepth Hc]".
-      destruct c' as [[|c'|]|]; try done.
-      iApply (join_spec with "Hc"). iNext. iIntros "* Hret".
-      by rewrite tctx_interp_singleton. }
-    iIntros (r); simpl_subst. iApply type_delete; [solve_typing..|].
-    iApply type_jump; solve_typing.
+    eapply type_fn; [solve_typing|]=> _ ??[?[]]. simpl_subst. via_tr_impl.
+    { iApply type_deref; [solve_extract|solve_typing..|]. intro_subst_as (j).
+      iApply type_delete; [solve_extract|done..|].
+      iApply (type_let' +[_ ◁ join_handle _] (λ r, +[r ◁ box retty])
+        (λ post '-[Φ], ∀a: 𝔄, Φ a → post -[a])).
+      { iIntros (??[?[]]) "_ _ _ _ _ $$ /=[j _] Obs". rewrite tctx_hasty_val.
+        iDestruct "j" as (?) "[_ join]". case j as [[|j|]|]=>//.
+        iDestruct "join" as (?->) "join". iApply (join_spec with "join"). iNext.
+        iIntros (?) "fut". iDestruct ("fut" $! _) as (??) "(?&? & Obs')".
+        iCombine "Obs Obs'" as "?". iExists -[_].
+        rewrite right_id tctx_hasty_val. iSplit; [iExists _; by iFrame|].
+        iApply proph_obs_impl; [|done]=>/= ?[Imp ?]. by apply Imp. }
+      intro_subst. iApply type_jump; [solve_typing|solve_extract|solve_typing]. }
+    by move=>/= ?[?[]].
   Qed.
-*)
 End spawn.
 
 Global Hint Resolve join_handle_leak join_handle_real
